Rename picks to transmap where appropriate

src/generation_update_next.v
@@ -275,46 +275,47 @@ We need
 - To be able to do an ∧ or a ∗ over the transformation functions.
 *)
 
-Section picks.
+Section transmap.
   Context `{Σ : gFunctors}.
 
-  (** [Picks] contains transformation functions for a subset of ghost names. It is
+  (** [TransMap] contains transformation functions for a subset of ghost names. It is
   the entries that we have picked generational transformations for. *)
-  Definition Picks : Type := ∀ i, gmap gname (T Σ i).
+  Definition TransMap : Type := ∀ i, gmap gname (T Σ i).
 
-  Implicit Types (picks : Picks).
+  Implicit Types (transmap : TransMap).
 
   #[global]
-  Instance picks_subseteq : SubsetEq Picks :=
+  Instance transmap_subseteq : SubsetEq TransMap :=
     λ p1 p2, ∀ i, p1 i ⊆ p2 i.
 
   #[global]
-  Instance picks_subseteq_partialorder : PartialOrder picks_subseteq.
+  Instance transmap_subseteq_partialorder : PartialOrder transmap_subseteq.
   Proof.
     split.
   Admitted.
 
   #[global]
-  Instance picks_union : Union Picks :=
+  Instance transmap_union : Union TransMap :=
     λ p1 p2 i, p1 i ∪ p2 i.
 
-  Lemma picks_union_subseteq_l picks1 picks2 :
-    picks1 ⊆ picks1 ∪ picks2.
+  Lemma transmap_union_subseteq_l transmap1 transmap2 :
+    transmap1 ⊆ transmap1 ∪ transmap2.
   Proof. intros ?. apply map_union_subseteq_l. Qed.
 
-  (** Every pick in [picks] is a valid generational transformation and satisfies
+  (** Every pick in [transmap] is a valid generational transformation and satisfies
   the conditions for that cmra in [Ω]. *)
-  Definition picks_valid (picks : Picks) :=
-    ∀ i γ t, picks i !! γ = Some t → GenTrans t.
+  Definition transmap_valid (transmap : TransMap) :=
+    ∀ i γ t, transmap i !! γ = Some t → GenTrans t.
 
-  (** Build a global generational transformation based on the picks in [picks]. *)
-  Definition build_trans (picks : Picks) : (iResUR Σ → iResUR Σ) :=
+  (** Build a global generational transformation based on the transformations
+  * in [transmap]. *)
+  Definition build_trans (transmap : TransMap) : (iResUR Σ → iResUR Σ) :=
     λ (m : iResUR Σ) (i : gid Σ),
       map_imap (λ γ a,
-        (* If the map of picks contains a transformation then we apply the
+        (* If the map of transmap contains a transformation then we apply the
          * transformation. If no pick exists then we return the elemment
          * unchanged. Hence, we default to the identity transformation. *)
-        match picks i !! γ with
+        match transmap i !! γ with
         | Some picked_gt => Some $ map_unfold $ picked_gt $ map_fold a
         | None => Some a
         end
@@ -324,10 +325,10 @@ Section picks.
   Proof. done. Qed.
 
   #[global]
-  Lemma build_trans_generation picks :
-    picks_valid picks → GenTrans (build_trans picks).
+  Lemma build_trans_generation transmap :
+    transmap_valid transmap → GenTrans (build_trans transmap).
   Proof.
-    intros picksGT.
+    intros transmapGT.
     rewrite /build_trans.
     split.
     - rewrite /Proper.
@@ -335,8 +336,8 @@ Section picks.
       rewrite 2!map_lookup_imap.
       specialize (eq i γ).
       destruct eq as [a b eq|]; simpl; last done.
-      destruct (picks i !! γ) eqn:look.
-      * apply picksGT in look as [gt ?]. solve_proper.
+      destruct (transmap i !! γ) eqn:look.
+      * apply transmapGT in look as [gt ?]. solve_proper.
       * solve_proper.
     - intros ?? Hval.
       intros i γ.
@@ -344,11 +345,11 @@ Section picks.
       specialize (Hval i γ).
       destruct (a i !! γ) eqn:eq; rewrite eq /=; last done.
       rewrite eq in Hval.
-      destruct (picks i !! γ) as [pick|] eqn:eq2.
+      destruct (transmap i !! γ) as [pick|] eqn:eq2.
       * apply Some_validN.
         apply: cmra_morphism_validN.
         apply Some_validN.
-        specialize (picksGT i γ pick eq2) as [??].
+        specialize (transmapGT i γ pick eq2) as [??].
         apply generation_valid.
         apply: cmra_morphism_validN.
         apply Hval.
@@ -364,10 +365,10 @@ Section picks.
       destruct (m i !! γ) as [a|] eqn:look; rewrite look; simpl; last done.
       simpl.
       rewrite core_Some_pcore.
-      destruct (picks i !! γ) as [pick|] eqn:pickLook; simpl.
+      destruct (transmap i !! γ) as [pick|] eqn:pickLook; simpl.
       * rewrite core_Some_pcore.
         rewrite -cmra_morphism_pcore.
-        specialize (picksGT i γ pick pickLook) as ?.
+        specialize (transmapGT i γ pick pickLook) as ?.
         rewrite -generation_pcore.
         rewrite -(cmra_morphism_pcore map_fold).
         (* rewrite -cmra_morphism_pcore. *)
@@ -380,8 +381,8 @@ Section picks.
       rewrite !map_lookup_imap.
       rewrite 2!lookup_op.
       rewrite !map_lookup_imap.
-      destruct (picks i !! γ) as [pick|] eqn:pickLook.
-      * specialize (picksGT i γ pick pickLook) as ?.
+      destruct (transmap i !! γ) as [pick|] eqn:pickLook.
+      * specialize (transmapGT i γ pick pickLook) as ?.
         destruct (m1 i !! γ) eqn:eq1; destruct (m2 i !! γ) eqn:eq2;
           rewrite eq1 eq2; simpl; try done.
         rewrite -Some_op.
@@ -391,15 +392,15 @@ Section picks.
           rewrite eq1 eq2; simpl; try done.
   Qed.
 
-End picks.
+End transmap.
 
-Arguments Picks Σ : clear implicits.
+Arguments TransMap Σ : clear implicits.
 
 (* Definition of the next generation modality. *)
 Section promises.
   Context `{Σ : gFunctors}.
 
-  Implicit Types (picks : Picks Σ).
+  Implicit Types (transmap : TransMap Σ).
 
   (** Information about a promise _except_ for any information concerning its
    * dependencies. This lets us talk about a promise without having to talk
@@ -481,24 +482,24 @@ Section promises.
     - Merge two lists of promises.
    *)
 
-  Definition trans_at_deps picks (p : promise_info)
+  Definition trans_at_deps transmap (p : promise_info)
       (trans : deps_to_trans p.(pi_n) p.(pi_deps)) :=
     ∀ idx,
       let dep := p.(pi_deps) !!! idx
-      in picks dep.(psi_id) !! dep.(psi_γ) = Some (trans 👀 idx).
+      in transmap dep.(psi_id) !! dep.(psi_γ) = Some (trans 👀 idx).
 
-  (** The transformations in [picks] satisfy the relation in [p]. *)
-  Definition picks_satisfy_rel picks p :=
+  (** The transformations in [transmap] satisfy the relation in [p]. *)
+  Definition transmap_satisfy_rel transmap p :=
     ∃ trans t,
-      picks p.(pi_id) !! p.(pi_γ) = Some t ∧
-      trans_at_deps picks p trans ∧
+      transmap p.(pi_id) !! p.(pi_γ) = Some t ∧
+      trans_at_deps transmap p trans ∧
       p.(pi_rel) trans t.
 
-  (** The [picks] respect the promises in [ps]: There is a pick for every
+  (** The [transmap] respect the promises in [ps]: There is a pick for every
    * promise and all the relations in the promises are satisfied by the
-   * transformations in picks. *)
-  Definition picks_resp_promises picks (ps : list (promise_info)) :=
-    ∀ i p, ps !! i = Some p → picks_satisfy_rel picks p.
+   * transformations in transmap. *)
+  Definition transmap_resp_promises transmap (ps : list (promise_info)) :=
+    ∀ i p, ps !! i = Some p → transmap_satisfy_rel transmap p.
 
   Definition promises_unique (promises : list promise_info) : Prop :=
     ∀ i j p1 p2, i ≠ j → promises !! i = Some p1 → promises !! j = Some p2 →
@@ -557,11 +558,11 @@ Section promises.
         eexists _, (S i). done.
   Qed.
 
-  Lemma picks_satisfy_well_formed_cons p promises picks :
+  Lemma transmap_satisfy_well_formed_cons p promises transmap :
     promises_well_formed (p :: promises) →
-    picks_resp_promises picks promises →
+    transmap_resp_promises transmap promises →
     ∃ ts,
-      trans_at_deps picks p ts ∧
+      trans_at_deps transmap p ts ∧
       deps_preds_hold p.(pi_deps) ts.
   Proof.
     intros WF resp.
@@ -571,7 +572,7 @@ Section promises.
       (λ i x,
         let pd := p.(pi_deps) !!! i in
         pd.(psi_pred) x ∧
-        picks (psi_id pd) !! psi_γ pd = Some x))
+        transmap (psi_id pd) !! psi_γ pd = Some x))
       as (ts & ?).
     { intros di.
       destruct (hasDeps di) as (p' & j & look & ->).
@@ -607,24 +608,24 @@ Section promises.
   Definition promise_map_well_formed (pm : ∀ i, gmap gname promise_info) : Prop :=
     ∀ i γ p, (pm i) !! γ = Some p → p.(pi_id) = i ∧ p.(pi_γ) = γ.
 
-  (* TODO: We need to store evidence that the picks in [picks] satisfies the
+  (* TODO: We need to store evidence that the picks in [transmap] satisfies the
    * relations and predicates in the [promises]. *)
 
-  Equations picks_insert_go picks (id : gid Σ) (γ : gname) (pick : T Σ id)
+  Equations transmap_insert_go transmap (id : gid Σ) (γ : gname) (pick : T Σ id)
     (id' : gid Σ) : gmap gname (T Σ id') :=
-  | picks, _, γ, pick, id', with decide (id = id') => {
-    | left eq_refl => <[ γ := pick ]>(picks id')
-    | right _ => picks id'
+  | transmap, _, γ, pick, id', with decide (id = id') => {
+    | left eq_refl => <[ γ := pick ]>(transmap id')
+    | right _ => transmap id'
   }.
 
-  Definition picks_insert picks id γ pick : Picks Σ :=
-    picks_insert_go picks id γ pick.
+  Definition transmap_insert transmap id γ pick : TransMap Σ :=
+    transmap_insert_go transmap id γ pick.
 
-  Lemma picks_insert_lookup picks id γ t  :
-    (picks_insert picks id γ t) id !! γ = Some t.
+  Lemma transmap_insert_lookup transmap id γ t  :
+    (transmap_insert transmap id γ t) id !! γ = Some t.
   Proof.
-    rewrite /picks_insert.
-    rewrite picks_insert_go_equation_1.
+    rewrite /transmap_insert.
+    rewrite transmap_insert_go_equation_1.
     destruct (decide (id = id)) as [eq | neq]; last congruence.
     assert (eq = eq_refl) as ->.
     { rewrite (proof_irrel eq eq_refl). done. }
@@ -632,30 +633,30 @@ Section promises.
     rewrite lookup_insert. done.
   Qed.
 
-  Lemma picks_insert_lookup_ne picks id1 γ1 t id2 γ2 :
+  Lemma transmap_insert_lookup_ne transmap id1 γ1 t id2 γ2 :
     id1 ≠ id2 ∨ γ1 ≠ γ2 →
-    (picks_insert picks id1 γ1 t) id2 !! γ2 = picks id2 !! γ2.
+    (transmap_insert transmap id1 γ1 t) id2 !! γ2 = transmap id2 !! γ2.
   Proof.
     intros neq.
-    rewrite /picks_insert.
-    rewrite picks_insert_go_equation_1.
+    rewrite /transmap_insert.
+    rewrite transmap_insert_go_equation_1.
     destruct (decide (id1 = id2)) as [eq | neq2]; last done.
     destruct neq as [neq | neq]; first congruence.
     subst. simpl.
     rewrite lookup_insert_ne; done.
   Qed.
 
-  Lemma picks_insert_subseteq_r i γ t picks1 picks2 :
-    picks1 i !! γ = None →
-    picks1 ⊆ picks2 →
-    picks1 ⊆ picks_insert picks2 i γ t.
+  Lemma transmap_insert_subseteq_r i γ t transmap1 transmap2 :
+    transmap1 i !! γ = None →
+    transmap1 ⊆ transmap2 →
+    transmap1 ⊆ transmap_insert transmap2 i γ t.
   Proof.
     intros look sub.
     intros i'.
     apply map_subseteq_spec => γ' t' look'.
     destruct (decide (i = i' ∧ γ = γ')) as [[-> ->]|Hneq].
     - congruence.
-    - rewrite picks_insert_lookup_ne.
+    - rewrite transmap_insert_lookup_ne.
       * specialize (sub i').
         rewrite map_subseteq_spec in sub.
         apply sub.
@@ -663,11 +664,11 @@ Section promises.
       * apply not_and_r in Hneq; done.
   Qed.
 
-  Lemma picks_resp_promises_cons picks p promises :
-    picks_resp_promises picks promises ∧ picks_satisfy_rel picks p ↔
-    picks_resp_promises picks (p :: promises).
+  Lemma transmap_resp_promises_cons transmap p promises :
+    transmap_resp_promises transmap promises ∧ transmap_satisfy_rel transmap p ↔
+    transmap_resp_promises transmap (p :: promises).
   Proof.
-    rewrite /picks_resp_promises. split.
+    rewrite /transmap_resp_promises. split.
     - intros [all sat] [|n'] p'; simpl.
       * intros [= ->]. apply sat.
       * apply all.
@@ -676,18 +677,18 @@ Section promises.
       * apply (all 0). done.
   Qed.
 
-  Lemma picks_resp_promises_insert p promises picks t :
+  Lemma transmap_resp_promises_insert p promises transmap t :
     promises_well_formed (p :: promises) →
-    picks_resp_promises picks promises →
-    picks_resp_promises (picks_insert picks (pi_id p) (pi_γ p) t) promises.
+    transmap_resp_promises transmap promises →
+    transmap_resp_promises (transmap_insert transmap (pi_id p) (pi_γ p) t) promises.
   Proof.
     intros [[uniq hasDeps] WF] resp idx p2 look.
-    rewrite /picks_satisfy_rel.
+    rewrite /transmap_satisfy_rel.
     specialize (resp idx p2 look).
     destruct resp as (t' & ts & hi).
     exists t', ts.
     rewrite /trans_at_deps.
-    setoid_rewrite picks_insert_lookup_ne.
+    setoid_rewrite transmap_insert_lookup_ne.
     + apply hi.
     + apply (uniq idx p2 look).
     + specialize (
@@ -699,14 +700,14 @@ Section promises.
       apply uniq.
   Qed.
 
-  Definition picks_overlap_resp_promises picks (ps : list (promise_info)) :=
+  Definition transmap_overlap_resp_promises transmap (ps : list (promise_info)) :=
     ∀ i p, ps !! i = Some p →
-      picks_satisfy_rel picks p ∨ (picks p.(pi_id) !! p.(pi_γ) = None).
+      transmap_satisfy_rel transmap p ∨ (transmap p.(pi_id) !! p.(pi_γ) = None).
 
-  Lemma trans_at_deps_subseteq picks1 picks2 p ts :
-    picks1 ⊆ picks2 →
-    trans_at_deps picks1 p ts →
-    trans_at_deps picks2 p ts.
+  Lemma trans_at_deps_subseteq transmap1 transmap2 p ts :
+    transmap1 ⊆ transmap2 →
+    trans_at_deps transmap1 p ts →
+    trans_at_deps transmap2 p ts.
   Proof.
     intros sub ta.
     intros idx. simpl.
@@ -717,34 +718,34 @@ Section promises.
     apply ta.
   Qed.
 
-  Lemma picks_overlap_resp_promises_cons picks p promises :
-    picks_overlap_resp_promises picks (p :: promises) →
-    picks_overlap_resp_promises picks promises.
+  Lemma transmap_overlap_resp_promises_cons transmap p promises :
+    transmap_overlap_resp_promises transmap (p :: promises) →
+    transmap_overlap_resp_promises transmap promises.
   Proof. intros HL. intros i ? look. apply (HL (S i) _ look). Qed.
 
- Lemma picks_promises_to_maps picks (promises : list promise_info) :
-    picks_overlap_resp_promises picks promises →
+ Lemma transmap_promises_to_maps transmap (promises : list promise_info) :
+    transmap_overlap_resp_promises transmap promises →
     promises_well_formed promises →
-    ∃ (map : Picks Σ),
-      picks_resp_promises map promises ∧
-      picks ⊆ map.
+    ∃ (map : TransMap Σ),
+      transmap_resp_promises map promises ∧
+      transmap ⊆ map.
   Proof.
     induction promises as [|p promises' IH].
-    - intros _. exists picks.
+    - intros _. exists transmap.
       split; last done.
       intros ? ?. inversion 1.
     - intros HR [WF WF'].
       specialize (promise_well_formed_neq_deps _ _ WF) as depsDiff.
       destruct IH as (map & resp & sub).
-      {  eapply picks_overlap_resp_promises_cons. done. } { done. }
+      {  eapply transmap_overlap_resp_promises_cons. done. } { done. }
       (* We either need to use the transformation in [picks] or extract one
        * from [p]. *)
-      destruct (picks p.(pi_id) !! p.(pi_γ)) eqn:look.
+      destruct (transmap p.(pi_id) !! p.(pi_γ)) eqn:look.
       + destruct (HR 0 p) as [sat | ?]; [done | | congruence].
         destruct sat as (ts & t & transIn & hold & pRelHolds).
         exists map. (* We don't insert as map already has transformation. *)
         split; last done.
-        apply picks_resp_promises_cons. split; try done.
+        apply transmap_resp_promises_cons. split; try done.
         eexists _, _. split_and!; last done.
         -- specialize (sub p.(pi_id)).
            rewrite map_subseteq_spec in sub.
@@ -752,68 +753,68 @@ Section promises.
            done.
         -- eapply trans_at_deps_subseteq; done.
       + eassert _ as sat.
-        { eapply picks_satisfy_well_formed_cons; done. }
+        { eapply transmap_satisfy_well_formed_cons; done. }
         destruct sat as (ts & transIn & hold).
         eassert (∃ t, _) as [t pRelHolds].
         { apply p.(pi_witness). apply hold. }
-        exists (picks_insert map p.(pi_id) p.(pi_γ) t).
+        exists (transmap_insert map p.(pi_id) p.(pi_γ) t).
         split.
-        * apply picks_resp_promises_cons.
+        * apply transmap_resp_promises_cons.
           split.
-          -- apply picks_resp_promises_insert; done.
-          -- rewrite /picks_satisfy_rel.
+          -- apply transmap_resp_promises_insert; done.
+          -- rewrite /transmap_satisfy_rel.
             exists ts, t.
-            split. { by rewrite picks_insert_lookup. }
+            split. { by rewrite transmap_insert_lookup. }
             split; last done.
             intros ??.
-            rewrite picks_insert_lookup_ne; first apply transIn.
+            rewrite transmap_insert_lookup_ne; first apply transIn.
             apply depsDiff.
-        * apply picks_insert_subseteq_r; done.
+        * apply transmap_insert_subseteq_r; done.
   Qed.
 
   Lemma promises_to_maps (promises : list promise_info) :
     promises_well_formed promises →
-    ∃ (picks : Picks Σ), picks_resp_promises picks promises.
+    ∃ (transmap : TransMap Σ), transmap_resp_promises transmap promises.
   Proof.
     intros WF.
-    edestruct (picks_promises_to_maps (λ i : gid Σ, ∅)) as [m [resp a]].
+    edestruct (transmap_promises_to_maps (λ i : gid Σ, ∅)) as [m [resp a]].
     2: { done. }
     - intros ???. right. done.
     - exists m. apply resp.
   Qed.
 
-  (* Turn a map of picks and a list of promises into a full map of picks. *)
-  Definition build_full_promises picks (ps : list (promise_info)) : Picks Σ :=
-    λ id, ∅.
-    (* λ id, *)
-    (*   foldl (λ p m, *)
-    (*     if (id = p.(pi_id)) *)
-    (*     then <[ p.(pi_γ) := p.(pi_) ] *)
-    (*   ) (ø) ps. *)
+  (* (* Turn a map of picks and a list of promises into a full map of picks. *) *)
+  (* Definition build_full_promises picks (ps : list (promise_info)) : TransMap Σ := *)
+  (*   λ id, ∅. *)
+  (*   (* λ id, *) *)
+  (*   (*   foldl (λ p m, *) *)
+  (*   (*     if (id = p.(pi_id)) *) *)
+  (*   (*     then <[ p.(pi_γ) := p.(pi_) ] *) *)
+  (*   (*   ) (ø) ps. *) *)
 
   (* (* TODO: This is the key result that we want to prove. *) *)
   (* Lemma build_full_properties picks ps : *)
   (*   let gt := build_full_promises picks ps *)
-  (*   in picks ⊆ gt ∧ picks_resp_promises gt ps. *)
+  (*   in picks ⊆ gt ∧ transmap_resp_promises gt ps. *)
   (* Proof. *)
   (* Admitted. *)
 
   (* NOTE: This is not possible! We need to feed the picks into the promises as
   * the resulting transformation can depend on the picks. *)
   (* TODO: This is the key result we want to prove. *)
-  Lemma map_from_picks_promises picks promises :
+  Lemma map_from_transmap_promises transmap promises :
     promises_well_formed promises →
-    ∃ (map : Picks Σ),
-      picks_resp_promises map promises ∧
-      picks ⊆ map.
+    ∃ (map : TransMap Σ),
+      transmap_resp_promises map promises ∧
+      transmap ⊆ map.
   Proof.
     intros WF.
     edestruct (promises_to_maps) as (mapP & resp); first done.
-    exists (picks ∪ mapP).
-    split; last apply picks_union_subseteq_l.
+    exists (transmap ∪ mapP).
+    split; last apply transmap_union_subseteq_l.
     intros ? p look.
     destruct (resp i _ look) as (ts & t & ? & ? & ?).
-    destruct (picks p.(pi_id) !! p.(pi_γ)) as [t2|] eqn:look2.
+    destruct (transmap p.(pi_id) !! p.(pi_γ)) as [t2|] eqn:look2.
     - eexists _, t2.
       admit.
     - exists ts, t.
@@ -832,7 +833,7 @@ Arguments promise_self_info Σ : clear implicits.
 Section next_gen_definition.
   Context `{Σ : gFunctors}.
 
-  Implicit Types (picks : Picks Σ).
+  Implicit Types (picks : TransMap Σ).
 
   (* The resource [m] contains the agreement resources for all the picks in
   [picks]. *)
@@ -872,8 +873,8 @@ Section next_gen_definition.
       (* We own resources for everything in [picks] and [promises]. *)
       own_picks picks ∗ own_promises ps ∗
       ⌜ promises_well_formed ps ⌝ ∗
-      ∀ full_picks (val : picks_valid full_picks),
-        ⌜ picks_resp_promises full_picks ps ⌝ ∗
+      ∀ full_picks (val : transmap_valid full_picks),
+        ⌜ transmap_resp_promises full_picks ps ⌝ ∗
         ⌜ picks ⊆ full_picks ⌝ ∗
         let _ := build_trans_generation full_picks val in (* Why is this instance not found automatically? *)
         ⚡={build_trans full_picks}=> P.
@@ -883,14 +884,14 @@ End next_gen_definition.
 Notation "⚡==> P" := (nextgen P)
   (at level 99, P at level 200, format "⚡==>  P") : bi_scope.
 
-Section picks_properties.
+Section transmap_properties.
   Context {Σ : gFunctors}.
 
-  Lemma m_contains_tokens_for_picks_empty :
+  Lemma m_contains_tokens_for_transmap_empty :
     m_contains_tokens_for_picks (λ i : gid Σ, ∅) ε.
   Proof. done. Qed.
 
-End picks_properties.
+End transmap_properties.
 
 (* Ownership over generational ghost state. *)
 
@@ -1003,7 +1004,7 @@ Section rules.
     iExists (λ i, ∅), [].
     iSplitL "".
     { iExists ε. rewrite ownM_unit' left_id. iPureIntro.
-      apply m_contains_tokens_for_picks_empty. }
+      apply m_contains_tokens_for_transmap_empty. }
     iSplit; first done.
     iSplit; first done.
     iIntros (full_picks).
